<?xml version="1.0"?>
<rdf:RDF xmlns="https://github.com/Bianca-LM/art-criticism-ontology/mat#"
     xml:base="https://github.com/Bianca-LM/art-criticism-ontology/mat"
     xmlns:dc="http://purl.org/dc/elements/1.1/"
     xmlns:mat="https://github.com/Bianca-LM/art-criticism-ontology/mat#"
     xmlns:owl="http://www.w3.org/2002/07/owl#"
     xmlns:rdf="http://www.w3.org/1999/02/22-rdf-syntax-ns#"
     xmlns:xml="http://www.w3.org/XML/1998/namespace"
     xmlns:xsd="http://www.w3.org/2001/XMLSchema#"
     xmlns:opla="http://ontologydesignpatterns.org/opla/"
     xmlns:rdfs="http://www.w3.org/2000/01/rdf-schema#"
     xmlns:opla1="http://www.ontologydesignpatterns.org/opla/"
     xmlns:terms="http://purl.org/dc/terms/"
     xmlns:arco-dd="https://w3id.org/arco/ontology/denotative-description/1.2#"
     xmlns:catalogue="https://w3id.org/arco/ontology/catalogue/">
    <owl:Ontology rdf:about="https://github.com/Bianca-LM/art-criticism-ontology/mat">
        <owl:versionIRI rdf:resource="https://github.com/Bianca-LM/art-criticism-ontology/1.0"/>
        <owl:imports rdf:resource="https://w3id.org/arco/ontology/denotative-description/1.2"/>
        <dc:creator>Bianca La Manna</dc:creator>
        <dc:title>OM&amp;TA (Ontology of Material &amp; Techniques in Art)</dc:title>
        <terms:license>CC BY 4.0</terms:license>
        <rdfs:comment>OM&amp;TA (Ontology of Materials &amp; Techniques in Art) is an ontology which aims at representing the relationship between materials and techniques for the description of artworks in a semantic way.</rdfs:comment>
    </owl:Ontology>
    


    <!-- 
    ///////////////////////////////////////////////////////////////////////////////////////
    //
    // Object Properties
    //
    ///////////////////////////////////////////////////////////////////////////////////////
     -->

    


    <!-- https://github.com/Bianca-LM/art-criticism-ontology/mat#hasDecoration -->

    <owl:ObjectProperty rdf:about="https://github.com/Bianca-LM/art-criticism-ontology/mat#hasDecoration">
        <rdfs:domain rdf:resource="https://github.com/Bianca-LM/art-criticism-ontology/mat#Artwork"/>
        <rdfs:range rdf:resource="https://github.com/Bianca-LM/art-criticism-ontology/mat#Decoration"/>
        <rdfs:comment>The property connects the artwork to its decoration</rdfs:comment>
    </owl:ObjectProperty>
    


    <!-- https://github.com/Bianca-LM/art-criticism-ontology/mat#hasDecorativeTechnique -->

    <owl:ObjectProperty rdf:about="https://github.com/Bianca-LM/art-criticism-ontology/mat#hasDecorativeTechnique">
        <rdfs:subPropertyOf rdf:resource="https://github.com/Bianca-LM/art-criticism-ontology/mat#hasTechnique"/>
        <rdfs:domain rdf:resource="https://github.com/Bianca-LM/art-criticism-ontology/mat#Decoration"/>
        <rdfs:range rdf:resource="http://www.w3.org/TR/2004/REC-xmlschema-2-20041028/Decorative_Technique"/>
        <rdfs:comment>The property connects the decoration that belongs to an artwork to the decorative technique used to realize it.</rdfs:comment>
    </owl:ObjectProperty>
    


    <!-- https://github.com/Bianca-LM/art-criticism-ontology/mat#hasFrame -->

    <owl:ObjectProperty rdf:about="https://github.com/Bianca-LM/art-criticism-ontology/mat#hasFrame">
        <rdfs:domain rdf:resource="https://github.com/Bianca-LM/art-criticism-ontology/mat#Artwork"/>
        <rdfs:range rdf:resource="https://github.com/Bianca-LM/art-criticism-ontology/mat#Frame"/>
        <rdfs:comment>The property connects the artwork to its frame</rdfs:comment>
    </owl:ObjectProperty>
    


    <!-- https://github.com/Bianca-LM/art-criticism-ontology/mat#hasInscription -->

    <owl:ObjectProperty rdf:about="https://github.com/Bianca-LM/art-criticism-ontology/mat#hasInscription">
        <rdfs:domain rdf:resource="https://github.com/Bianca-LM/art-criticism-ontology/mat#Artwork"/>
        <rdfs:range>
            <owl:Class>
                <owl:oneOf rdf:parseType="Collection">
                    <rdf:Description rdf:about="https://github.com/Bianca-LM/art-criticism-ontology/mat/Inscription"/>
                </owl:oneOf>
            </owl:Class>
        </rdfs:range>
        <rdfs:comment>The property connects the artwork to its inscription</rdfs:comment>
    </owl:ObjectProperty>
    


    <!-- https://github.com/Bianca-LM/art-criticism-ontology/mat#hasOrnament -->

    <owl:ObjectProperty rdf:about="https://github.com/Bianca-LM/art-criticism-ontology/mat#hasOrnament">
        <rdfs:domain rdf:resource="https://github.com/Bianca-LM/art-criticism-ontology/mat#Artwork"/>
        <rdfs:range rdf:resource="https://github.com/Bianca-LM/art-criticism-ontology/mat#Ornament"/>
        <rdfs:comment>The property connects the artwork to its ornament</rdfs:comment>
    </owl:ObjectProperty>
    


    <!-- https://github.com/Bianca-LM/art-criticism-ontology/mat#hasOrnamentalTechnique -->

    <owl:ObjectProperty rdf:about="https://github.com/Bianca-LM/art-criticism-ontology/mat#hasOrnamentalTechnique">
        <rdfs:subPropertyOf rdf:resource="https://github.com/Bianca-LM/art-criticism-ontology/mat#hasTechnique"/>
        <rdfs:domain rdf:resource="https://github.com/Bianca-LM/art-criticism-ontology/mat#Ornament"/>
        <rdfs:range rdf:resource="http://www.w3.org/TR/2004/REC-xmlschema-2-20041028/Ornamental_Technique"/>
        <rdfs:comment>The property connects the ornament that belongs to an artwork to the ornamental technique that has been used to realize it.</rdfs:comment>
    </owl:ObjectProperty>
    


    <!-- https://github.com/Bianca-LM/art-criticism-ontology/mat#hasSupport -->

    <owl:ObjectProperty rdf:about="https://github.com/Bianca-LM/art-criticism-ontology/mat#hasSupport">
        <rdfs:subPropertyOf rdf:resource="http://www.w3.org/2002/07/owl#topObjectProperty"/>
        <rdfs:domain rdf:resource="https://github.com/Bianca-LM/art-criticism-ontology/mat#Artwork"/>
        <rdfs:range>
            <owl:Class>
                <owl:oneOf rdf:parseType="Collection">
                    <rdf:Description rdf:about="https://github.com/Bianca-LM/art-criticism-ontology/mat/Current_Support"/>
                </owl:oneOf>
            </owl:Class>
        </rdfs:range>
        <rdfs:comment>The property connects the artwork to its current support</rdfs:comment>
    </owl:ObjectProperty>
    


    <!-- https://github.com/Bianca-LM/art-criticism-ontology/mat#hasTechnique -->

    <owl:ObjectProperty rdf:about="https://github.com/Bianca-LM/art-criticism-ontology/mat#hasTechnique">
        <rdfs:domain rdf:resource="https://github.com/Bianca-LM/art-criticism-ontology/mat#Artwork"/>
        <rdfs:range rdf:resource="https://github.com/Bianca-LM/art-criticism-ontology/mat#Technique"/>
        <rdfs:comment>The property connects the artwork to the technique used to realize it</rdfs:comment>
    </owl:ObjectProperty>
    


    <!-- https://github.com/Bianca-LM/art-criticism-ontology/mat#isDated -->

    <owl:ObjectProperty rdf:about="https://github.com/Bianca-LM/art-criticism-ontology/mat#isDated">
        <rdfs:domain>
            <owl:Class>
                <owl:oneOf rdf:parseType="Collection">
                    <rdf:Description rdf:about="https://github.com/Bianca-LM/art-criticism-ontology/mat/Signature"/>
                </owl:oneOf>
            </owl:Class>
        </rdfs:domain>
        <rdfs:range>
            <owl:Class>
                <owl:oneOf rdf:parseType="Collection">
                    <rdf:Description rdf:about="https://github.com/Bianca-LM/art-criticism-ontology/mat/Signature_Datation"/>
                </owl:oneOf>
            </owl:Class>
        </rdfs:range>
        <rdfs:comment>The property connects the signature to its datation, if it is written on the artwork itself.</rdfs:comment>
    </owl:ObjectProperty>
    


    <!-- https://github.com/Bianca-LM/art-criticism-ontology/mat#isMadeOf -->

    <owl:ObjectProperty rdf:about="https://github.com/Bianca-LM/art-criticism-ontology/mat#isMadeOf">
        <rdfs:domain rdf:resource="https://github.com/Bianca-LM/art-criticism-ontology/mat#Frame"/>
        <rdfs:domain rdf:resource="https://github.com/Bianca-LM/art-criticism-ontology/mat#Support"/>
        <rdfs:range rdf:resource="https://github.com/Bianca-LM/art-criticism-ontology/mat#Material"/>
        <rdfs:comment>The property connects the frame and the support to the material which they are made of.</rdfs:comment>
    </owl:ObjectProperty>
    


    <!-- https://github.com/Bianca-LM/art-criticism-ontology/mat#isMarked -->

    <owl:ObjectProperty rdf:about="https://github.com/Bianca-LM/art-criticism-ontology/mat#isMarked">
        <rdfs:domain rdf:resource="https://github.com/Bianca-LM/art-criticism-ontology/mat#Artwork"/>
        <rdfs:range rdf:resource="https://github.com/Bianca-LM/art-criticism-ontology/mat#Mark"/>
        <rdfs:range rdf:resource="https://github.com/Bianca-LM/art-criticism-ontology/mat#Mark_of_Carter"/>
        <rdfs:range rdf:resource="https://github.com/Bianca-LM/art-criticism-ontology/mat#Mark_of_Founder"/>
        <rdfs:comment>The property connects the artwork to the mark that has been affixed on it.</rdfs:comment>
    </owl:ObjectProperty>
    


    <!-- https://github.com/Bianca-LM/art-criticism-ontology/mat#isMountedOn -->

    <owl:ObjectProperty rdf:about="https://github.com/Bianca-LM/art-criticism-ontology/mat#isMountedOn">
        <rdfs:subPropertyOf rdf:resource="https://github.com/Bianca-LM/art-criticism-ontology/mat#hasSupport"/>
        <rdfs:domain rdf:resource="https://github.com/Bianca-LM/art-criticism-ontology/mat#Material"/>
        <rdfs:range>
            <owl:Class>
                <owl:oneOf rdf:parseType="Collection">
                    <rdf:Description rdf:about="https://github.com/Bianca-LM/art-criticism-ontology/mat/Current_Support"/>
                </owl:oneOf>
            </owl:Class>
        </rdfs:range>
        <rdfs:comment>The property connects the material on which the artwork has been realised to the current support on which it is mounted</rdfs:comment>
    </owl:ObjectProperty>
    


    <!-- https://github.com/Bianca-LM/art-criticism-ontology/mat#isPerformedOn -->

    <owl:ObjectProperty rdf:about="https://github.com/Bianca-LM/art-criticism-ontology/mat#isPerformedOn">
        <rdfs:domain rdf:resource="https://github.com/Bianca-LM/art-criticism-ontology/mat#Technique"/>
        <rdfs:range rdf:resource="https://github.com/Bianca-LM/art-criticism-ontology/mat#Material"/>
        <rdfs:comment>The property connects the technique to the material it is performed on.</rdfs:comment>
    </owl:ObjectProperty>
    


    <!-- https://github.com/Bianca-LM/art-criticism-ontology/mat#isSigned -->

    <owl:ObjectProperty rdf:about="https://github.com/Bianca-LM/art-criticism-ontology/mat#isSigned">
        <rdfs:domain rdf:resource="https://github.com/Bianca-LM/art-criticism-ontology/mat#Artwork"/>
        <rdfs:range>
            <owl:Class>
                <owl:oneOf rdf:parseType="Collection">
                    <rdf:Description rdf:about="https://github.com/Bianca-LM/art-criticism-ontology/mat/Signature"/>
                </owl:oneOf>
            </owl:Class>
        </rdfs:range>
        <rdfs:comment>The property connects the artwork to the signature of the artist that made it.</rdfs:comment>
    </owl:ObjectProperty>
    


    <!-- https://github.com/Bianca-LM/art-criticism-ontology/mat#transferredFrom -->

    <owl:ObjectProperty rdf:about="https://github.com/Bianca-LM/art-criticism-ontology/mat#transferredFrom">
        <rdfs:domain>
            <owl:Class>
                <owl:unionOf rdf:parseType="Collection">
                    <owl:Class>
                        <owl:oneOf rdf:parseType="Collection">
                            <rdf:Description rdf:about="https://github.com/Bianca-LM/art-criticism-ontology/mat/Current_Support"/>
                        </owl:oneOf>
                    </owl:Class>
                    <owl:Class>
                        <owl:oneOf rdf:parseType="Collection">
                            <rdf:Description rdf:about="https://github.com/Bianca-LM/art-criticism-ontology/mat/Previous_Support"/>
                        </owl:oneOf>
                    </owl:Class>
                </owl:unionOf>
            </owl:Class>
        </rdfs:domain>
        <rdfs:range>
            <owl:Class>
                <owl:oneOf rdf:parseType="Collection">
                    <rdf:Description rdf:about="https://github.com/Bianca-LM/art-criticism-ontology/mat/Previous_Support"/>
                </owl:oneOf>
            </owl:Class>
        </rdfs:range>
        <rdfs:comment>The property connects the current support of an artwork to the previous support from which it has been transferred.</rdfs:comment>
    </owl:ObjectProperty>
    


    <!-- 
    ///////////////////////////////////////////////////////////////////////////////////////
    //
    // Data properties
    //
    ///////////////////////////////////////////////////////////////////////////////////////
     -->

    


    <!-- https://github.com/Bianca-LM/art-criticism-ontology/mat#dateOfSignature -->

    <owl:DatatypeProperty rdf:about="https://github.com/Bianca-LM/art-criticism-ontology/mat#dateOfSignature">
        <rdfs:domain>
            <owl:Class>
                <owl:oneOf rdf:parseType="Collection">
                    <rdf:Description rdf:about="https://github.com/Bianca-LM/art-criticism-ontology/mat/Signature_Datation"/>
                </owl:oneOf>
            </owl:Class>
        </rdfs:domain>
        <rdfs:range rdf:resource="http://www.w3.org/2001/XMLSchema#dateTime"/>
        <rdfs:comment>The property represents the date of the signature datation</rdfs:comment>
    </owl:DatatypeProperty>
    


    <!-- https://github.com/Bianca-LM/art-criticism-ontology/mat#hasInscriptionContent -->

    <owl:DatatypeProperty rdf:about="https://github.com/Bianca-LM/art-criticism-ontology/mat#hasInscriptionContent">
        <rdfs:domain>
            <owl:Class>
                <owl:oneOf rdf:parseType="Collection">
                    <rdf:Description rdf:about="https://github.com/Bianca-LM/art-criticism-ontology/mat/Inscription"/>
                </owl:oneOf>
            </owl:Class>
        </rdfs:domain>
        <rdfs:range rdf:resource="http://www.w3.org/2000/01/rdf-schema#Literal"/>
        <rdfs:comment>This property represents the content of an inscription.</rdfs:comment>
    </owl:DatatypeProperty>
    


    <!-- https://github.com/Bianca-LM/art-criticism-ontology/mat#hasSignature -->

    <owl:DatatypeProperty rdf:about="https://github.com/Bianca-LM/art-criticism-ontology/mat#hasSignature">
        <rdfs:domain>
            <owl:Class>
                <owl:oneOf rdf:parseType="Collection">
                    <rdf:Description rdf:about="https://github.com/Bianca-LM/art-criticism-ontology/mat/Signature"/>
                </owl:oneOf>
            </owl:Class>
        </rdfs:domain>
        <rdfs:range rdf:resource="http://www.w3.org/2000/01/rdf-schema#Literal"/>
        <rdfs:comment>This property represents the signature of the artist imposed on the artwork.</rdfs:comment>
    </owl:DatatypeProperty>
    


    <!-- 
    ///////////////////////////////////////////////////////////////////////////////////////
    //
    // Classes
    //
    ///////////////////////////////////////////////////////////////////////////////////////
     -->

    


    <!-- http://www.w3.org/TR/2004/REC-xmlschema-2-20041028/Decorative_Technique -->

    <owl:Class rdf:about="http://www.w3.org/TR/2004/REC-xmlschema-2-20041028/Decorative_Technique">
        <rdfs:subClassOf rdf:resource="https://github.com/Bianca-LM/art-criticism-ontology/mat#Technique"/>
        <rdfs:comment>A technique that traditionally is used  for the creation of decorative elements.</rdfs:comment>
    </owl:Class>
    


    <!-- http://www.w3.org/TR/2004/REC-xmlschema-2-20041028/External_Physical_Datum -->

    <owl:Class rdf:about="http://www.w3.org/TR/2004/REC-xmlschema-2-20041028/External_Physical_Datum">
        <rdfs:comment>Every external physical datum of an artwork.</rdfs:comment>
    </owl:Class>
    


    <!-- http://www.w3.org/TR/2004/REC-xmlschema-2-20041028/Ornamental_Technique -->

    <owl:Class rdf:about="http://www.w3.org/TR/2004/REC-xmlschema-2-20041028/Ornamental_Technique">
        <rdfs:subClassOf rdf:resource="https://github.com/Bianca-LM/art-criticism-ontology/mat#Technique"/>
        <rdfs:comment>A technique that traditionally is used for the creation of ornaments.</rdfs:comment>
    </owl:Class>
    


    <!-- https://github.com/Bianca-LM/art-criticism-ontology/mat#Artwork -->

    <owl:Class rdf:about="https://github.com/Bianca-LM/art-criticism-ontology/mat#Artwork">
        <rdfs:comment>The entity which represents the work of art</rdfs:comment>
    </owl:Class>
    


    <!-- https://github.com/Bianca-LM/art-criticism-ontology/mat#Artwork_Component -->

    <owl:Class rdf:about="https://github.com/Bianca-LM/art-criticism-ontology/mat#Artwork_Component">
        <rdfs:comment>A subcomponent of an artwork which can have its own material and technique.</rdfs:comment>
    </owl:Class>
    


    <!-- https://github.com/Bianca-LM/art-criticism-ontology/mat#Decoration -->

    <owl:Class rdf:about="https://github.com/Bianca-LM/art-criticism-ontology/mat#Decoration">
        <rdfs:subClassOf rdf:resource="https://github.com/Bianca-LM/art-criticism-ontology/mat#Artwork_Component"/>
        <owl:disjointWith rdf:resource="https://github.com/Bianca-LM/art-criticism-ontology/mat#Ornament"/>
        <rdfs:comment>An additional element which is main purpose is not practical or aesthetic, but brings &quot;decorum&quot; to another element.</rdfs:comment>
    </owl:Class>
    


    <!-- https://github.com/Bianca-LM/art-criticism-ontology/mat#Frame -->

    <owl:Class rdf:about="https://github.com/Bianca-LM/art-criticism-ontology/mat#Frame">
        <rdfs:subClassOf rdf:resource="http://www.w3.org/TR/2004/REC-xmlschema-2-20041028/External_Physical_Datum"/>
        <rdfs:comment>Some works of art comes with a frame, which has a material and can  have a decoration.</rdfs:comment>
    </owl:Class>
    


    <!-- https://github.com/Bianca-LM/art-criticism-ontology/mat#Mark -->

    <owl:Class rdf:about="https://github.com/Bianca-LM/art-criticism-ontology/mat#Mark">
        <owl:equivalentClass rdf:resource="https://w3id.org/arco/ontology/denotative-description/Brand"/>
        <rdfs:subClassOf rdf:resource="https://github.com/Bianca-LM/art-criticism-ontology/mat#Artwork_Component"/>
        <rdfs:comment>The sign of an external contribution out of the author. It can be the founder or the carter, mainly used with scultpures.</rdfs:comment>
    </owl:Class>
    


    <!-- https://github.com/Bianca-LM/art-criticism-ontology/mat#Mark_of_Carter -->

    <owl:Class rdf:about="https://github.com/Bianca-LM/art-criticism-ontology/mat#Mark_of_Carter">
        <rdfs:subClassOf rdf:resource="https://github.com/Bianca-LM/art-criticism-ontology/mat#Mark"/>
        <rdfs:comment>The mark of a workshop or factory for model plasters.</rdfs:comment>
    </owl:Class>
    


    <!-- https://github.com/Bianca-LM/art-criticism-ontology/mat#Mark_of_Founder -->

    <owl:Class rdf:about="https://github.com/Bianca-LM/art-criticism-ontology/mat#Mark_of_Founder">
        <rdfs:subClassOf rdf:resource="https://github.com/Bianca-LM/art-criticism-ontology/mat#Mark"/>
        <rdfs:comment>The mark of a workshop or factory for casting metal.</rdfs:comment>
    </owl:Class>
    


    <!-- https://github.com/Bianca-LM/art-criticism-ontology/mat#Material -->

    <owl:Class rdf:about="https://github.com/Bianca-LM/art-criticism-ontology/mat#Material">
        <rdfs:subClassOf rdf:resource="http://www.w3.org/TR/2004/REC-xmlschema-2-20041028/External_Physical_Datum"/>
        <rdfs:comment>It is the proper material on which the work of art has been made. It can be different from the support.</rdfs:comment>
    </owl:Class>
    


    <!-- https://github.com/Bianca-LM/art-criticism-ontology/mat#Ornament -->

    <owl:Class rdf:about="https://github.com/Bianca-LM/art-criticism-ontology/mat#Ornament">
        <rdfs:subClassOf rdf:resource="https://github.com/Bianca-LM/art-criticism-ontology/mat#Artwork_Component"/>
        <rdfs:comment>An additional element other from the main body of the artwork, which helps through repeated patterns, and natural elements at the visual organization of the artwork, in which prevails the aesthetic function.</rdfs:comment>
    </owl:Class>
    


    <!-- https://github.com/Bianca-LM/art-criticism-ontology/mat#Support -->

    <owl:Class rdf:about="https://github.com/Bianca-LM/art-criticism-ontology/mat#Support">
        <rdfs:subClassOf rdf:resource="http://www.w3.org/TR/2004/REC-xmlschema-2-20041028/External_Physical_Datum"/>
        <rdfs:comment>The support on which the technique is performed, &quot;given from nature or elaborated by human beings&quot; (Sciolla).</rdfs:comment>
    </owl:Class>
    


    <!-- https://github.com/Bianca-LM/art-criticism-ontology/mat#Technique -->

    <owl:Class rdf:about="https://github.com/Bianca-LM/art-criticism-ontology/mat#Technique">
        <rdfs:comment>&quot;The union of all the principles, rules and manners elaborated by the artists for the material processing over time, experimented in the workshops and artistic laboratories&quot; as defined by Sciolla.</rdfs:comment>
    </owl:Class>
    


    <!-- https://w3id.org/arco/ontology/denotative-description/Brand -->

    <rdf:Description rdf:about="https://w3id.org/arco/ontology/denotative-description/Brand">
        <rdfs:subClassOf rdf:resource="https://github.com/Bianca-LM/art-criticism-ontology/mat#Artwork_Component"/>
    </rdf:Description>
    


    <!-- 
    ///////////////////////////////////////////////////////////////////////////////////////
    //
    // Individuals
    //
    ///////////////////////////////////////////////////////////////////////////////////////
     -->

    


    <!-- https://github.com/Bianca-LM/art-criticism-ontology/mat/Current_Support -->

    <owl:NamedIndividual rdf:about="https://github.com/Bianca-LM/art-criticism-ontology/mat/Current_Support">
        <rdf:type rdf:resource="https://github.com/Bianca-LM/art-criticism-ontology/mat#Support"/>
        <transferredFrom rdf:resource="https://github.com/Bianca-LM/art-criticism-ontology/mat/Previous_Support"/>
        <rdfs:comment>The current support, which can be different from the original support for different reasons (restoration, demages, transfer etc.).</rdfs:comment>
    </owl:NamedIndividual>
    <rdf:Description>
        <rdf:type rdf:resource="http://www.w3.org/2002/07/owl#NegativePropertyAssertion"/>
        <owl:sourceIndividual rdf:resource="https://github.com/Bianca-LM/art-criticism-ontology/mat/Current_Support"/>
        <owl:assertionProperty rdf:resource="https://github.com/Bianca-LM/art-criticism-ontology/mat#transferredFrom"/>
        <owl:targetIndividual rdf:resource="https://github.com/Bianca-LM/art-criticism-ontology/mat/Current_Support"/>
    </rdf:Description>
    


    <!-- https://github.com/Bianca-LM/art-criticism-ontology/mat/Inscription -->

    <owl:NamedIndividual rdf:about="https://github.com/Bianca-LM/art-criticism-ontology/mat/Inscription">
        <rdf:type rdf:resource="https://github.com/Bianca-LM/art-criticism-ontology/mat#Artwork_Component"/>
        <hasInscriptionContent rdf:datatype="http://www.w3.org/2000/01/rdf-schema#Literal"></hasInscriptionContent>
        <rdfs:comment>Every kind of text added to the work of art.</rdfs:comment>
    </owl:NamedIndividual>
    


    <!-- https://github.com/Bianca-LM/art-criticism-ontology/mat/Previous_Support -->

    <owl:NamedIndividual rdf:about="https://github.com/Bianca-LM/art-criticism-ontology/mat/Previous_Support">
        <rdf:type rdf:resource="https://github.com/Bianca-LM/art-criticism-ontology/mat#Support"/>
        <transferredFrom rdf:resource="https://github.com/Bianca-LM/art-criticism-ontology/mat/Previous_Support"/>
        <rdfs:comment>The original support used by the artist.</rdfs:comment>
    </owl:NamedIndividual>
    <rdf:Description>
        <rdf:type rdf:resource="http://www.w3.org/2002/07/owl#NegativePropertyAssertion"/>
        <owl:sourceIndividual rdf:resource="https://github.com/Bianca-LM/art-criticism-ontology/mat/Previous_Support"/>
        <owl:assertionProperty rdf:resource="https://github.com/Bianca-LM/art-criticism-ontology/mat#transferredFrom"/>
        <owl:targetIndividual rdf:resource="https://github.com/Bianca-LM/art-criticism-ontology/mat/Current_Support"/>
    </rdf:Description>
    


    <!-- https://github.com/Bianca-LM/art-criticism-ontology/mat/Signature -->

    <owl:NamedIndividual rdf:about="https://github.com/Bianca-LM/art-criticism-ontology/mat/Signature">
        <rdf:type rdf:resource="https://github.com/Bianca-LM/art-criticism-ontology/mat#Artwork_Component"/>
        <isDated rdf:resource="https://github.com/Bianca-LM/art-criticism-ontology/mat/Signature_Datation"/>
        <hasSignature rdf:datatype="http://www.w3.org/2000/01/rdf-schema#Literal"></hasSignature>
        <rdfs:comment>The signature of the author left on the artwork itself.</rdfs:comment>
    </owl:NamedIndividual>
    


    <!-- https://github.com/Bianca-LM/art-criticism-ontology/mat/Signature_Datation -->

    <owl:NamedIndividual rdf:about="https://github.com/Bianca-LM/art-criticism-ontology/mat/Signature_Datation">
        <rdf:type rdf:resource="https://github.com/Bianca-LM/art-criticism-ontology/mat#Artwork_Component"/>
        <dateOfSignature rdf:datatype="http://www.w3.org/2001/XMLSchema#dateTime"></dateOfSignature>
        <rdfs:comment>The datation of the signature left by the author on the artwork itself.</rdfs:comment>
    </owl:NamedIndividual>
</rdf:RDF>



<!-- Generated by the OWL API (version 4.5.9.2019-02-01T07:24:44Z) https://github.com/owlcs/owlapi -->

