@prefix : <https://github.com/Bianca-LM/art-criticism-ontology/mat#> .
@prefix dc: <http://purl.org/dc/elements/1.1/> .
@prefix mat: <https://github.com/Bianca-LM/art-criticism-ontology/mat#> .
@prefix owl: <http://www.w3.org/2002/07/owl#> .
@prefix rdf: <http://www.w3.org/1999/02/22-rdf-syntax-ns#> .
@prefix xml: <http://www.w3.org/XML/1998/namespace> .
@prefix xsd: <http://www.w3.org/2001/XMLSchema#> .
@prefix opla: <http://www.ontologydesignpatterns.org/opla/> .
@prefix rdfs: <http://www.w3.org/2000/01/rdf-schema#> .
@prefix terms: <http://purl.org/dc/terms/> .
@prefix arco-dd: <https://w3id.org/arco/ontology/denotative-description/1.2#> .
@prefix catalogue: <https://w3id.org/arco/ontology/catalogue/> .
@base <https://github.com/Bianca-LM/art-criticism-ontology/mat> .

<https://github.com/Bianca-LM/art-criticism-ontology/mat> rdf:type owl:Ontology ;
                                                           owl:versionIRI <https://github.com/Bianca-LM/art-criticism-ontology/1.0> ;
                                                           owl:imports <https://w3id.org/arco/ontology/denotative-description/1.2> ;
                                                           dc:creator "Bianca La Manna" ;
                                                           dc:title "OM&TA (Ontology of Material & Techniques in Art)" ;
                                                           terms:license "CC BY 4.0" ;
                                                           rdfs:comment "OM&TA (Ontology of Materials & Techniques in Art) is an ontology which aims at representing the relationship between materials and techniques for the description of artworks in a semantic way." .

#################################################################
#    Object Properties
#################################################################

###  https://github.com/Bianca-LM/art-criticism-ontology/mat#hasAuthor
mat:hasAuthor rdf:type owl:ObjectProperty ;
              owl:equivalentProperty <https://w3id.org/arco/ontology/context-description/hasAuthor> ;
              rdfs:domain mat:Artwork ;
              rdfs:range mat:Author ;
              rdfs:comment "This property connects the artwork to the author who made it." ;
              rdfs:label "has author"@en .


###  https://github.com/Bianca-LM/art-criticism-ontology/mat#hasCurrentSupport
mat:hasCurrentSupport rdf:type owl:ObjectProperty ;
                      rdfs:subPropertyOf mat:hasSupport ;
                      owl:inverseOf mat:isCurrentSupportOf ;
                      rdfs:domain mat:Artwork ;
                      rdfs:range mat:Support ;
                      rdfs:comment "This property connects an artwork to its current support." ;
                      rdfs:label "has current support"@en .


###  https://github.com/Bianca-LM/art-criticism-ontology/mat#hasDecoration
mat:hasDecoration rdf:type owl:ObjectProperty ;
                  rdfs:domain mat:Artwork ;
                  rdfs:range mat:Decoration ;
                  rdfs:comment "The property connects the artwork to its decoration" ;
                  rdfs:label "has decoration"@en .


###  https://github.com/Bianca-LM/art-criticism-ontology/mat#hasDecorativeTechnique
mat:hasDecorativeTechnique rdf:type owl:ObjectProperty ;
                           rdfs:subPropertyOf mat:hasTechnique ;
                           rdfs:domain mat:Decoration ;
                           rdfs:range mat:Decorative_Technique ;
                           rdfs:comment "The property connects the decoration that belongs to an artwork to the decorative technique used to realize it." ;
                           rdfs:label "has decorative technique"@en .


###  https://github.com/Bianca-LM/art-criticism-ontology/mat#hasFrame
mat:hasFrame rdf:type owl:ObjectProperty ;
             rdfs:domain mat:Artwork ;
             rdfs:range mat:Frame ;
             rdfs:comment "The property connects the artwork to its frame" ;
             rdfs:label "has frame"@en .


###  https://github.com/Bianca-LM/art-criticism-ontology/mat#hasInscription
mat:hasInscription rdf:type owl:ObjectProperty ;
                   rdfs:domain mat:Artwork ;
                   rdfs:range mat:Inscription ;
                   rdfs:comment "The property connects the artwork to its inscription" ;
                   rdfs:label "has inscription"@en .


###  https://github.com/Bianca-LM/art-criticism-ontology/mat#hasOrnament
mat:hasOrnament rdf:type owl:ObjectProperty ;
                rdfs:domain mat:Artwork ;
                rdfs:range mat:Ornament ;
                rdfs:comment "The property connects the artwork to its ornament" ;
                rdfs:label "has ornament"@en .


###  https://github.com/Bianca-LM/art-criticism-ontology/mat#hasOrnamentalTechnique
mat:hasOrnamentalTechnique rdf:type owl:ObjectProperty ;
                           rdfs:subPropertyOf mat:hasTechnique ;
                           rdfs:domain mat:Ornament ;
                           rdfs:range mat:Ornamental_Technique ;
                           rdfs:comment "The property connects the ornament that belongs to an artwork to the ornamental technique that has been used to realize it." ;
                           rdfs:label "has ornamental technique"@en .


###  https://github.com/Bianca-LM/art-criticism-ontology/mat#hasPreviousSupport
mat:hasPreviousSupport rdf:type owl:ObjectProperty ;
                       rdfs:subPropertyOf mat:hasSupport ;
                       owl:inverseOf mat:isPreviousSupportOf ;
                       rdfs:domain mat:Artwork ;
                       rdfs:range mat:Support ;
                       rdfs:comment "This property connects the arttwork with its previous support." ;
                       rdfs:label "has previous support"@en .


###  https://github.com/Bianca-LM/art-criticism-ontology/mat#hasSupport
mat:hasSupport rdf:type owl:ObjectProperty ;
               rdfs:subPropertyOf owl:topObjectProperty ;
               rdfs:domain mat:Artwork ;
               rdfs:range mat:Support ;
               rdfs:comment "The property connects the artwork to its current support" ;
               rdfs:label "has support"@en .


###  https://github.com/Bianca-LM/art-criticism-ontology/mat#hasTechnique
mat:hasTechnique rdf:type owl:ObjectProperty ;
                 rdfs:domain mat:Artwork ;
                 rdfs:range mat:Technique ;
                 rdfs:comment "The property connects the artwork to the technique used to realize it" ;
                 rdfs:label "has technique"@en .


###  https://github.com/Bianca-LM/art-criticism-ontology/mat#hasTitle
mat:hasTitle rdf:type owl:ObjectProperty ;
             rdfs:domain mat:Artwork ;
             rdfs:range mat:Title ;
             rdfs:comment "This property connects the artwork with its official title."@en ;
             rdfs:label "has title"@en .


###  https://github.com/Bianca-LM/art-criticism-ontology/mat#isCurrentSupportOf
mat:isCurrentSupportOf rdf:type owl:ObjectProperty ;
                       rdfs:subPropertyOf mat:hasSupport ;
                       rdfs:domain mat:Support ;
                       rdfs:range mat:Artwork ;
                       rdfs:comment "Inverse property of mat:hasCurrentSupport" ;
                       rdfs:label "is current support of"@en .


###  https://github.com/Bianca-LM/art-criticism-ontology/mat#isDated
mat:isDated rdf:type owl:ObjectProperty ;
            rdfs:domain mat:Signature ;
            rdfs:range mat:Signature_Datation ;
            rdfs:comment "The property connects the signature to its datation, if it is written on the artwork itself." ;
            rdfs:label "is dated"@en .


###  https://github.com/Bianca-LM/art-criticism-ontology/mat#isMadeOf
mat:isMadeOf rdf:type owl:ObjectProperty ;
             rdfs:domain [ rdf:type owl:Class ;
                           owl:unionOf ( mat:Frame
                                         mat:Support
                                       )
                         ] ;
             rdfs:range mat:Material ;
             rdfs:comment "The property connects the frame and the support to the material which they are made of." ;
             rdfs:label "is made of"@en .


###  https://github.com/Bianca-LM/art-criticism-ontology/mat#isMarked
mat:isMarked rdf:type owl:ObjectProperty ;
             rdfs:domain mat:Artwork ;
             rdfs:range [ rdf:type owl:Class ;
                          owl:unionOf ( mat:Mark
                                        mat:Mark_of_Carter
                                        mat:Mark_of_Founder
                                      )
                        ] ;
             rdfs:comment "The property connects the artwork to the mark that has been affixed on it." ;
             rdfs:label "is marked"@en .


###  https://github.com/Bianca-LM/art-criticism-ontology/mat#isMountedOn
mat:isMountedOn rdf:type owl:ObjectProperty ;
                rdfs:subPropertyOf mat:hasSupport ;
                rdfs:domain mat:Material ;
                rdfs:range mat:Support ;
                rdfs:comment "The property connects the material on which the artwork has been realised to the current support on which it is mounted" ;
                rdfs:label "is mounted on"@en .


###  https://github.com/Bianca-LM/art-criticism-ontology/mat#isPerformedOn
mat:isPerformedOn rdf:type owl:ObjectProperty ;
                  rdfs:domain [ rdf:type owl:Class ;
                                owl:unionOf ( mat:Decorative_Technique
                                              mat:Ornamental_Technique
                                              mat:Technique
                                            )
                              ] ;
                  rdfs:range mat:Material ;
                  rdfs:comment "The property connects the technique to the material it is performed on." ;
                  rdfs:label "is performed on"@en .


###  https://github.com/Bianca-LM/art-criticism-ontology/mat#isPreviousSupportOf
mat:isPreviousSupportOf rdf:type owl:ObjectProperty ;
                        rdfs:subPropertyOf mat:hasSupport ;
                        rdfs:domain mat:Support ;
                        rdfs:range mat:Artwork ;
                        rdfs:comment "Inverse property of mat:hasPreviousSupport" ;
                        rdfs:label "is previous support of"@en .


###  https://github.com/Bianca-LM/art-criticism-ontology/mat#isSigned
mat:isSigned rdf:type owl:ObjectProperty ;
             rdfs:domain mat:Artwork ;
             rdfs:range mat:Signature ;
             rdfs:comment "The property connects the artwork to the signature of the artist that made it." ;
             rdfs:label "is signed"@en .


###  https://github.com/Bianca-LM/art-criticism-ontology/mat#transferredFrom
mat:transferredFrom rdf:type owl:ObjectProperty ;
                    rdfs:domain mat:Support ;
                    rdfs:range mat:Support ;
                    rdfs:comment "The property connects the current support of an artwork to the previous support from which it has been transferred." ;
                    rdfs:label "transferred from"@en .


###  https://w3id.org/arco/ontology/context-description/hasAuthor

#################################################################
#    Data properties
#################################################################

###  https://github.com/Bianca-LM/art-criticism-ontology/mat#dateOfSignature
mat:dateOfSignature rdf:type owl:DatatypeProperty ;
                    rdfs:range rdfs:Literal ;
                    rdfs:comment "The property represents the date of the signature datation" ;
                    rdfs:label "date of signature"@en .


###  https://github.com/Bianca-LM/art-criticism-ontology/mat#hasInscriptionContent
mat:hasInscriptionContent rdf:type owl:DatatypeProperty ;
                          rdfs:range rdfs:Literal ;
                          rdfs:comment "This property represents the content of an inscription." ;
                          rdfs:label "has inscription content"@en .


###  https://github.com/Bianca-LM/art-criticism-ontology/mat#hasSignature
mat:hasSignature rdf:type owl:DatatypeProperty ;
                 rdfs:range rdfs:Literal ;
                 rdfs:comment "This property represents the signature of the artist imposed on the artwork." ;
                 rdfs:label "has signature"@en .


#################################################################
#    Classes
#################################################################

###  https://github.com/Bianca-LM/art-criticism-ontology/mat#Artwork
mat:Artwork rdf:type owl:Class ;
            rdfs:comment "The entity which represents the work of art" ;
            rdfs:label "Artwork"@en .


###  https://github.com/Bianca-LM/art-criticism-ontology/mat#Artwork_Component
mat:Artwork_Component rdf:type owl:Class ;
                      rdfs:comment "A subcomponent of an artwork which can have its own material and technique." ;
                      rdfs:label "Artwork Component"@en .


###  https://github.com/Bianca-LM/art-criticism-ontology/mat#Author
mat:Author rdf:type owl:Class ;
           rdfs:comment "The artists who made the artwork" ;
           rdfs:label "Author"@en .


###  https://github.com/Bianca-LM/art-criticism-ontology/mat#Decoration
mat:Decoration rdf:type owl:Class ;
               rdfs:subClassOf mat:Artwork_Component ;
               owl:disjointWith mat:Ornament ;
               rdfs:comment "An additional element which is main purpose is not practical or aesthetic, but brings \"decorum\" to another element." ;
               rdfs:label "Decoration"@en .


###  https://github.com/Bianca-LM/art-criticism-ontology/mat#Decorative_Technique
mat:Decorative_Technique rdf:type owl:Class ;
                         rdfs:subClassOf mat:Technique ;
                         rdfs:comment "A technique that traditionally is used  for the creation of decorative elements." ;
                         rdfs:label "Decorative Technique"@en .


###  https://github.com/Bianca-LM/art-criticism-ontology/mat#External_Physical_Datum
mat:External_Physical_Datum rdf:type owl:Class ;
                            rdfs:comment "Every external physical datum of an artwork." ;
                            rdfs:label "External Physical Datum"@en .


###  https://github.com/Bianca-LM/art-criticism-ontology/mat#Frame
mat:Frame rdf:type owl:Class ;
          rdfs:subClassOf mat:External_Physical_Datum ;
          rdfs:comment "Some works of art comes with a frame, which has a material and can  have a decoration." ;
          rdfs:label "Frame"@en .


###  https://github.com/Bianca-LM/art-criticism-ontology/mat#Inscription
mat:Inscription rdf:type owl:Class ;
                rdfs:subClassOf mat:Artwork_Component ;
                rdfs:comment "Any kind of text added to the artwork, which is not a signature, a date or a mark." ;
                rdfs:label "Inscription"@en .


###  https://github.com/Bianca-LM/art-criticism-ontology/mat#Mark
mat:Mark rdf:type owl:Class ;
         owl:equivalentClass <https://w3id.org/arco/ontology/denotative-description/Brand> ;
         rdfs:subClassOf mat:Artwork_Component ;
         rdfs:comment "The sign of an external contribution out of the author. It can be the founder or the carter, mainly used with scultpures." ;
         rdfs:label "Mark"@en .


###  https://github.com/Bianca-LM/art-criticism-ontology/mat#Mark_of_Carter
mat:Mark_of_Carter rdf:type owl:Class ;
                   rdfs:subClassOf mat:Mark ;
                   rdfs:comment "The mark of a workshop or factory for model plasters." ;
                   rdfs:label "Mark of Carter"@en .


###  https://github.com/Bianca-LM/art-criticism-ontology/mat#Mark_of_Founder
mat:Mark_of_Founder rdf:type owl:Class ;
                    rdfs:subClassOf mat:Mark ;
                    rdfs:comment "The mark of a workshop or factory for casting metal." ;
                    rdfs:label "Mark of Founder"@en .


###  https://github.com/Bianca-LM/art-criticism-ontology/mat#Material
mat:Material rdf:type owl:Class ;
             rdfs:subClassOf mat:External_Physical_Datum ;
             rdfs:comment "It is the proper material on which the work of art has been made. It can be different from the support." ;
             rdfs:label "Material"@en .


###  https://github.com/Bianca-LM/art-criticism-ontology/mat#Ornament
mat:Ornament rdf:type owl:Class ;
             rdfs:subClassOf mat:Artwork_Component ;
             rdfs:comment "An additional element other from the main body of the artwork, which helps through repeated patterns, and natural elements at the visual organization of the artwork, in which prevails the aesthetic function." ;
             rdfs:label "Ornament"@en .


###  https://github.com/Bianca-LM/art-criticism-ontology/mat#Ornamental_Technique
mat:Ornamental_Technique rdf:type owl:Class ;
                         rdfs:subClassOf mat:Technique ;
                         rdfs:comment "A technique that traditionally is used for the creation of ornaments." ;
                         rdfs:label "Ornamental Technique"@en .


###  https://github.com/Bianca-LM/art-criticism-ontology/mat#Signature
mat:Signature rdf:type owl:Class ;
              rdfs:subClassOf mat:Artwork_Component ;
              rdfs:comment "The signature lived by the author on the artwork" ;
              rdfs:label "Signature"@en .


###  https://github.com/Bianca-LM/art-criticism-ontology/mat#Signature_Datation
mat:Signature_Datation rdf:type owl:Class ;
                       rdfs:subClassOf mat:Signature ;
                       rdfs:comment "The date of  the signature, lived by the authors themselves on the artwork." ;
                       rdfs:label "Signature Datation"@en .


###  https://github.com/Bianca-LM/art-criticism-ontology/mat#Support
mat:Support rdf:type owl:Class ;
            rdfs:subClassOf mat:External_Physical_Datum ;
            rdfs:comment "The support on which the technique is performed, \"given from nature or elaborated by human beings\" (Sciolla)." ;
            rdfs:label "Support"@en .


###  https://github.com/Bianca-LM/art-criticism-ontology/mat#Technique
mat:Technique rdf:type owl:Class ;
              rdfs:comment "\"The union of all the principles, rules and manners elaborated by the artists for the material processing over time, experimented in the workshops and artistic laboratories\" as defined by Sciolla." ;
              rdfs:label "Technique"@en .


###  https://github.com/Bianca-LM/art-criticism-ontology/mat#Title
mat:Title rdf:type owl:Class ;
          rdfs:comment "The title given by the author to the artwork" ;
          rdfs:label "Title"@en .


###  https://w3id.org/arco/ontology/denotative-description/Brand
<https://w3id.org/arco/ontology/denotative-description/Brand> rdfs:subClassOf mat:Artwork_Component .


###  Generated by the OWL API (version 4.5.9.2019-02-01T07:24:44Z) https://github.com/owlcs/owlapi
